\begin{align}
    c^T_t &= y^T_t - (1 - I_t)L(y^T_t) + I_t(q_t d_{t+1} - d_t), \\
    (1 - I_t)d_{t+1} &= 0, \\
    \lambda_t &= U'(A(c^T_t, F(h_t)))A_1(c_t^T, F(h_t)),\\
    (1-\tau_t^d)q_t^d \lambda_t &= \beta E_t \lambda_{t+1}, \\
    I_t(q^d_t - q_t) &= 0, \\
    \frac{A_2(c_t^T, F(h_t))}{A_1(c_t^t, F(h_t))} &= \frac{w_t}{F'(h_t)} , \\
   w_t &\ge \gamma\frac{w_{t-1}}{\epsilon_t},\\
   h_t &\le \bar{h},\\
   \left( h_t - \bar{h} \right) \left( w_t - \gamma\frac{w_{t-1}}{\epsilon_t}\right) &= 0, \\
    I_t \left[ q_t - \frac{E_t I_{t+1}}{1+r^*} \right] &= 0,
\end{align}